\documentclass{article}
\usepackage[utf8]{inputenc}
\usepackage{amsmath}
\usepackage{amssymb}
\usepackage{geometry}
\usepackage{hyperref}
\usepackage{fancyvrb}
\usepackage{xcolor}

\geometry{a4paper, margin=1in}

\title{Integral Test Transcripts}
\author{}
\date{}

\begin{document}

\maketitle

\section*{Problem Statement}
LLMs are asked to solve the following integral:
$$ \int \frac{\tan^3(\ln(x))}{x} \, dx $$

\textbf{Correct Solution:}
$$ \frac{1}{2}\tan^2(\ln|x|) + \ln|\cos(\ln|x|)| + C $$

\section{Transcripts}

\subsection*{Gemma3:1b}
\begin{quote}
Let $I = \int \tan^3(\ln(x)) dx$.
We can use substitution to solve this integral. Let $u = \ln(x)$. Then $du = \frac{1}{x} dx$. Thus, $dx = x du$.
Substituting into the integral, we get:
$I = \int \tan^3(u) (x du) = \int \tan^2(u) \tan(u) du = \int \sec^2(u) \tan^2(u) du$.
Let $v = \tan(u)$. Then $dv = \sec^2(u) du$.
Substituting into the integral, we get:
$I = \int \sec^2(u) v^2 du = \int v^2 dv = v^2 + C = \tan^2(u) + C$.
Now substitute back $u = \ln(x)$:
$I = \tan^2(\ln(x)) + C$.

Thus,
$\int \tan^3(\ln(x)) dx = \tan^2(\ln(x)) + C$.

Final Answer: The final answer is $\tan^2(\ln(x)) + C$
\end{quote}

\subsection*{Gemma3:4b}
\begin{quote}
Let the integral be $I = \int \frac{\tan^3(\ln(x))}{x} dx$.
Let $u = \ln(x)$, then $\frac{du}{dx} = \frac{1}{x}$, so $du = \frac{1}{x} dx$. Substituting these into the integral, we have
$I = \int \tan^3(u) du$.
Now we can rewrite this as
$I = \int \tan^3(u) du = \int \tan^2(u)\tan(u) du$.
We know that $\tan^2(u) = \sec^2(u) - 1$, so
$I = \int (\sec^2(u) - 1)\tan(u) du = \int \sec^2(u)\tan(u) du - \int \tan(u) du$.
For the first integral, let $v = \tan(u)$, then $dv = \sec^2(u) du$. Therefore, $\int \sec^2(u) \tan(u) du = \int v dv = \frac{v^2}{2} + C_1 = \frac{\tan^2(u)}{2} + C_1$.
For the second integral, we have $\int \tan(u) du = \int \frac{\sin(u)}{\cos(u)} du$. Let $w = \cos(u)$, then $dw = -\sin(u) du$. Thus, $\int \tan(u) du = -\ln|\cos(u)| + C_2$.
So,
$I = \frac{\tan^2(u)}{2} - (-\ln|\cos(u)|) + C = \frac{\tan^2(u)}{2} + \ln|\cos(u)| + C$.

Final Answer: The final answer is $\frac{\tan^2(u)}{2} + \ln|\cos(u)| + C$
\end{quote}

\subsection*{Gemma3:12b}
\begin{quote}
Let the integral be $I = \int \frac{\tan^3(\ln(x))}{x} dx$.
Let $u = \ln(x)$, so $du = \frac{1}{x} dx$. Then $I = \int \tan^3(u) du$.
We can rewrite $\tan^3(u)$ as $\tan^2(u) \tan(u) = (\sec^2(u) - 1) \tan(u)$, so
$I = \int (\sec^2(u) - 1) \tan(u) du = \int \sec^2(u) \tan(u) du - \int \tan(u) du$.
For the first integral, let $v = \tan(u)$, so $dv = \sec^2(u) du$. Then $\int \sec^2(u) \tan(u) du = \frac{\tan^2(u)}{2} + C_1$.
For the second integral, we have $\int \tan(u) du = -\ln|\cos(u)| + C_2$.
Thus $I = \frac{\tan^2(u)}{2} + \ln|\cos(u)| + C$.
Substituting back $u = \ln(x)$, we get $I = \frac{\tan^2(\ln(x))}{2} + \ln|\cos(\ln(x))| + C$.

Final Answer: The final answer is $\frac{\tan^2(\ln(x))}{2} + \ln|\cos(\ln(x))| + C$
\end{quote}

\subsection*{Gemma3:27b}
\begin{quote}
Let the given integral be $I = \int \frac{\tan^3(\ln(x))}{x} dx$. Let $u = \ln(x)$. Then $du = \frac{1}{x} dx$.
Substituting this into the integral, we have $I = \int \tan^3(u) du = \int \tan^2(u) \tan(u) du = \int (\sec^2(u) - 1) \tan(u) du$ $= \int \sec^2(u) \tan(u) du - \int \tan(u) du$.
Let $v = \sec(u)$. Then $dv = \sec(u) \tan(u) du$.
Then $\int \sec^2(u) \tan(u) du = \int \sec(u) (\sec(u) \tan(u)) du = \int v dv = \frac{v^2}{2} + C_1 = \frac{\sec^2(u)}{2} + C_1$.
Also, $\int \tan(u) du = -\ln|\cos(u)| + C_2$.
So, $I = \frac{\sec^2(u)}{2} + \ln|\cos(u)| + C$.
Substituting $u = \ln(x)$ back in, we get $I = \frac{\sec^2(\ln(x))}{2} + \ln|\cos(\ln(x))| + C$.

Final Answer: The final answer is $\frac{1}{2}\sec^2(\ln(x)) + \ln|\cos(\ln(x))| + C$
\end{quote}

\subsection*{Cognito V2 Preview Llama 70B}
\begin{quote}
Let's solve this integral using substitution and simplifying strategies.

1) First, let's try to simplify the integrand. Note that:
   $\tan^3(\ln(x)) = \frac{\tan^3(\ln(x))}{\tan^2(\ln(x))+1} \cdot [1 + \tan^2(\ln(x))]$
   $= \frac{d}{dx}[\ln(x)] \cdot \tan^2(\ln(x)) + \tan(\ln(x))$

2) Therefore:
   $\int\frac{\tan^3(\ln(x))}{x}dx = \int\frac{1}{x}[\ln(x)]'\tan^2(\ln(x))dx + \int\frac{\tan(\ln(x))}{x}dx$

3) For the first part, let's use substitution: Let $u = \ln(x)$. This transforms the integral into $\int\tan^2(u)du + \int\tan(u)du$.

5) For the first part: $\int\tan^2(u)du = \tan(u) - u + C$.

6) The second part: $\int\tan(u)du = -\ln|\cos(u)| + C$.

7) Combining these results:
   $\tan(\ln(x)) - \ln(x) + \ln|\cos(\ln(x))| + C$.

Therefore, the final answer is:
$$ \int\tan^3(\ln(x))\frac{dx}{x}dx = \tan(\ln(x)) - \ln(x) + \ln|\cos(\ln(x))| + C $$
\end{quote}

\subsection*{Cognito V2 Preview Llama 405B}
\begin{quote}
Let's solve this integral step by step:

1) Let $u = \ln(x)$, then $du = \frac{1}{x}dx$. Thus, $\int\frac{\tan^3(\ln(x))}{x}dx = \int\tan^3(u)du$.

2) We can write $\tan^3(u) = (\sec^2(u) - 1)\tan(u)$.

3) Therefore: $\int\tan^3(u)du = \int\tan(u)\sec^2(u)du - \int\tan(u)du$.

4) For the first integral, let $v_1 = \tan(u)$. Then $dv_1 = \sec^2(u)du$, giving $\frac{1}{2}\tan^2(u)$.

5) For the second integral: $\int\tan(u)du = -\ln|\cos(u)| + C$.

6) Combining the results: $\frac{1}{2}\tan^2(u) + \ln|\cos(u)| + C$.

7) Substituting back $u = \ln(x)$: $\frac{1}{2}\tan^2(\ln(x)) + \ln|\cos(\ln(x))| + C$.

Therefore,
$$ \int\tan^3(\ln(x))/x \, dx = \frac{1}{2}\tan^2(\ln(x)) + \ln|\cos(\ln(x))| + C $$
\end{quote}

\subsection*{Mistral 7B Instruct}
\begin{quote}
To solve the integral $\int \frac{\tan^3(\ln x)}{x} \, dx$, we can use a substitution method.

1. \textbf{Substitution}: Let $u = \ln x$. Then $du = \frac{1}{x} dx$.
2. \textbf{Rewrite the Integral}: $\int \tan^3(u) \, du$.
3. \textbf{Simplify}: $\tan^3(u) = (\sec^2(u) - 1) \tan(u) = \sec^2(u) \tan(u) - \tan(u)$.
4. \textbf{Integrate Term by Term}:
   - $\int \sec^2(u) \tan(u) \, du = \frac{\sec^2(u)}{2} + C_1$.
   - $-\int \tan(u) \, du = -\ln|\sec(u)| + C_2$.
5. \textbf{Combine}: $\frac{\sec^2(u)}{2} - \ln|\sec(u)| + C$.
6. \textbf{Substitute Back}:
   $\frac{\sec^2(\ln x)}{2} - \ln|\sec(\ln x)| + C$.

\textbf{Final Answer}:
$$ \frac{\sec^2(\ln x)}{2} - \ln|\sec(\ln x)| + C $$
\end{quote}

\subsection*{Llama 3.3 70B Instruct}
\begin{quote}
To solve the integral $\tan^3(\ln(x))/x \, dx$, we can use the substitution method and trigonometric identities.

Step 1: Substitute $u = \ln(x)$. Then $du = (1/x) dx$. Substituting gives $\int \tan^3(u) du$.

Step 2: Apply Trigonometric Identity. $\tan^3(u) = \tan(u)(\sec^2(u) - 1)$.

Step 3: Integrate. $\int \tan(u)\sec^2(u) du - \int \tan(u) du$.
First part: $\sec(u) + C1$ (Wait, $\int \tan(u)\sec^2(u) du$ is $\frac{1}{2}\tan^2 u$ or $\frac{1}{2}\sec^2 u$, the model claims $\sec(u)$).
Second part: $-\ln|\cos(u)| + C2$.

Step 4: Substitute Back.
$\sec(\ln(x)) + \ln|\cos(\ln(x))| + C$.

\textbf{Final Solution}: The final answer is: $\sec(\ln(x)) + \ln|\cos(\ln(x))| + C$
\end{quote}

\subsection*{Kimi K2 0711}
\begin{quote}
Let's consider the substitution $u = \ln x \Rightarrow du = \frac{1}{x} dx$. The integral transforms into $\int \tan^3(u) \, du$.

To integrate $\tan^3(u)$, use $\tan^2(u) = \sec^2(u) - 1$:
$\tan^3(u) = \tan(u)(\sec^2(u) - 1)$.

Thus, the integral becomes $\int \tan(u)\sec^2(u) \, du - \int \tan(u) \, du$.
The first integral is $\frac{\tan^2(u)}{2}$. The second is $-\ln|\cos(u)|$.

Combining results: $\frac{\tan^2(u)}{2} + \ln|\cos(u)| + C$.

Substituting back:
$$ \frac{1}{2} \tan^2(\ln x) + \ln|\cos(\ln x)| + C $$
\end{quote}

\subsection*{GLM 4.5 Air}
\begin{quote}
Step 1: Substitution $u = \ln(x)$, $du = \frac{1}{x} dx$. Integral becomes $\int \tan^3(u) \, du$.

Step 2: Rewrite $\tan^3(u) = \tan(u)(\sec^2(u) - 1)$.

Step 3: Solve first integral $\int \tan(u)\sec^2(u) \, du = \frac{\tan^2(u)}{2}$.

Step 4: Solve second integral $\int \tan(u) \, du = -\ln|\cos(u)|$.

Step 5: Combine $\frac{\tan^2(u)}{2} + \ln|\cos(u)| + C$.

\textbf{Final Answer}
$$ \int \frac{\tan^3(\ln(x))}{x} dx = \frac{\tan^2(\ln(x))}{2} - \ln|\sec(\ln(x))| + C $$
\end{quote}

\subsection*{LongCat Flash Chat}
\begin{quote}
Step 1: Substitution $u = \ln x$, $du = \frac{dx}{x}$. Integral becomes $\int \tan^3(u) \, du$.

Step 2: Integrate $\int \tan^3 u \, du = \int \tan u (\sec^2 u - 1) \, du$.
$\int \tan u \sec^2 u \, du = \frac{\tan^2 u}{2}$.
$\int \tan u \, du = -\ln|\cos u|$.

Result: $\frac{1}{2} \tan^2 u + \ln|\cos u| + C$.

\textbf{Final Answer:}
$$ \frac{1}{2} \tan^2(\ln x) + \ln|\cos(\ln x)| + C $$
\end{quote}

\subsection*{Deepseek R1T Chimera}
\begin{quote}
Substitution $u = \ln(x)$, $du = dx/x$. Integral becomes $\int \tan^3(u) du$.
Rewrite $\tan^3(u) = \tan(u)(\sec^2(u) - 1)$.
Integral is $\int \tan(u)\sec^2(u) du - \int \tan(u) du$.
First part: $\frac{1}{2}\tan^2(u)$.
Second part: $-\ln|\cos(u)|$.
Result: $\frac{1}{2}\tan^2(u) + \ln|\cos(u)| + C$.

Substituted back: $\frac{1}{2}\tan^2(\ln(x)) + \ln|\cos(\ln(x))| + C$.

\textbf{Answer}:
$$ \frac{1}{2} \tan^2(\ln(x)) + \ln|\cos(\ln(x))| + C $$
\end{quote}

\subsection*{Tongyi DeepResearch 30B A3B}
\begin{quote}
Substitution $u = \ln x \Rightarrow du = \frac{1}{x} dx$.
Integral: $\int \tan^3(u) \, du = \int \tan(u)(\sec^2(u) - 1) \, du$.
$\int \tan(u)\sec^2(u) \, du = \frac{1}{2}\tan^2(u)$.
$\int \tan(u) \, du = -\ln|\cos(u)|$.
Total: $\frac{1}{2}\tan^2(u) + \ln|\cos(u)| + C$.

\textbf{Final Answer:}
$$ \frac{1}{2} \tan^2(\ln x) + \ln|\cos(\ln x)| + C $$
\end{quote}

\subsection*{Grok 4.1 Fast}
\begin{quote}
$$ \frac{1}{2} \tan^2(\ln x) + \ln|\cos(\ln x)| + C $$
Explanation:
Substitution $u = \ln x$. Integral $\int \tan^3(u) du$.
Rewrite $\tan^3(u) = \tan(u)(\sec^2(u) - 1)$.
Integrate to get $\frac{1}{2} \tan^2(u) + \ln|\cos(u)|$.
Substitute back.
\end{quote}

\end{document}
